theories/Lambda/Rewrite/BottomUp.v
@@ -28,6 +28,7 @@ Require Import MirrorCore.Lambda.ExprUnify.
 Require Import MirrorCore.Lambda.AppN.
 Require Import MirrorCore.Lambda.ExprSubstitute.
 Require Import MirrorCore.Lambda.RewriteRelations.
+Require Import MirrorCore.Lambda.Rewrite.Core.
 
 Set Implicit Arguments.
 Set Strict Implicit.
@@ -68,201 +69,6 @@ Section setoid.
       RbaseD r t2 = Some rD2 ->
       t1 = t2.
 
-
-  (** This monad abstracts the idea of working under a context.
-   ** It is morally exactly the same as [rtac] except for two differences:
-   ** 1) It is generalized over the goal representation so it can avoid
-   **    manifesting [Goal]s
-   ** 2) It has an extra [tvs'] argument that allows it to avoid pushing
-   **    terms into the context when it does not need to.
-   **
-   ** TODO(gmalecha):
-   **   This should be unified with the [rtac] monad but understanding
-   **   the full design still requires a bit more work.
-   **)
-  Definition mrw (T : Type) : Type :=
-    tenv typ -> tenv typ -> tenv typ -> nat -> nat ->
-    forall c : Ctx typ (expr typ func), ctx_subst c ->
-                                        option (T * ctx_subst c).
-
-  Definition rw_ret {T} (val : T) : mrw T :=
-    fun _ _ _ _ _ _ s => Some (val, s).
-
-  Definition rw_bind {T U} (c : mrw T) (k : T -> mrw U) : mrw U :=
-    fun tvs' tus tvs nus nvs ctx cs =>
-      match c tvs' tus tvs nus nvs ctx cs with
-      | None => None
-      | Some (v,cs') => k v tvs' tus tvs nus nvs ctx cs'
-      end.
-
-  Definition rw_orelse {T} (c1 c2 : mrw T) : mrw T :=
-    fun tvs' tus tvs nus nvs ctx cs =>
-      match c1 tvs' tus tvs nus nvs ctx cs with
-      | None => c2 tvs' tus tvs nus nvs ctx cs
-      | z => z
-      end.
-
-  Definition rw_fail {T} : mrw T :=
-    fun tvs' tus tvs nus nvs ctx cs =>
-      None.
-
-  Definition rw_bind_catch {T U : Type} (c : mrw T) (k : T -> mrw U)
-             (otherwise : mrw U)
-  : mrw U :=
-    fun tus' tus tvs nus nvs ctx cs =>
-      match c tus' tus tvs nus nvs ctx cs with
-      | None => otherwise tus' tus tvs nus nvs ctx cs
-      | Some (val,cs') => k val tus' tus tvs nus nvs ctx cs'
-      end.
-
-  Lemma rw_orelse_case
-  : forall (T : Type) (A B : mrw T) a b c d e f g h,
-      @rw_orelse _ A B a b c d e f g = h ->
-      A a b c d e f g = h \/
-      B a b c d e f g = h.
-  Proof using.
-    unfold rw_orelse. intros.
-    forward.
-  Qed.
-
-  Lemma rw_bind_catch_case
-  : forall (T U : Type) (A : mrw T) (B : T -> mrw U) (C : mrw U)
-           a b c d e f g h,
-      @rw_bind_catch _ _ A B C a b c d e f g = h ->
-      (exists x g', A a b c d e f g = Some (x,g') /\
-                    B x a b c d e f g' = h) \/
-      (C a b c d e f g = h /\ A a b c d e f g = None).
-  Proof using.
-    unfold rw_bind_catch. intros; forward.
-    left. do 2 eexists; split; eauto.
-  Qed.
-
-  Lemma rw_bind_case
-  : forall (T U : Type) (A : mrw T) (B : T -> mrw U)
-           a b c d e f g h,
-      @rw_bind _ _ A B a b c d e f g = Some h ->
-      exists x g',
-        A a b c d e f g = Some (x, g') /\
-        B x a b c d e f g' = Some h.
-  Proof using.
-    unfold rw_bind. intros; forward.
-    do 2 eexists; eauto.
-  Qed.
-
-  Section rw_map2.
-    Context {T U V : Type}.
-    Variable f : T -> U -> mrw V.
-
-    Fixpoint rw_map2 (ts : list T) (us : list U) : mrw (list V) :=
-      match ts , us with
-        | nil , nil => rw_ret nil
-        | t :: ts , u :: us =>
-          rw_bind (f t u) (fun v =>
-                             rw_bind (rw_map2 ts us)
-                                     (fun vs => rw_ret (v :: vs)))
-        | _ , _ => rw_fail
-      end.
-  End rw_map2.
-
-  Definition mrw_equiv {T} (rT : T -> T -> Prop) (l : mrw T) (r : mrw T)
-  : Prop :=
-    forall a b c d e f g,
-      Roption (Eqpair rT eq) (l a b c d e f g) (r a b c d e f g).
-
-  Instance Reflexive_mrw_equiv {T} (rT : T -> T -> Prop)
-           {Refl_rT : Reflexive rT}
-  : Reflexive (mrw_equiv rT).
-  Proof using.
-    red. red. intros. eapply Reflexive_Roption. eapply Reflexive_Eqpair; eauto.
-  Qed.
-
-  Instance Symmetric_mrw_equiv {T} (rT : T -> T -> Prop)
-           {Sym_rT : Symmetric rT}
-  : Symmetric (mrw_equiv rT).
-  Proof using.
-    red. red. intros. eapply Symmetric_Roption. eapply Symmetric_Eqpair; eauto.
-    eapply H.
-  Qed.
-
-  Instance Transitive_mrw_equiv {T} (rT : T -> T -> Prop)
-           {Trans_rT : Transitive rT}
-  : Transitive (mrw_equiv rT).
-  Proof using.
-    red. red. intros. eapply Transitive_Roption.
-    eapply Transitive_Eqpair; eauto with typeclass_instances.
-    eapply H. eapply H0.
-  Qed.
-
-  Lemma rw_bind_assoc
-  : forall {T U V} (c : mrw T) (k : T -> mrw U) (k' : U -> mrw V),
-      mrw_equiv eq
-                (rw_bind (rw_bind c k) k')
-                (rw_bind c (fun x => rw_bind (k x) k')).
-  Proof using.
-    unfold rw_bind. simpl.
-    red. intros.
-    destruct (c a b c0 d e f g); try constructor.
-    destruct p.
-    eapply Reflexive_Roption. apply Reflexive_Eqpair; eauto.
-  Qed.
-
-  Lemma rw_bind_rw_ret
-  : forall {T U} (x : T) (k : T -> mrw U),
-      rw_bind (rw_ret x) k = k x.
-  Proof using. reflexivity. Qed.
-
-  Lemma rw_bind_rw_fail
-  : forall {T U} (k : T -> mrw U),
-      rw_bind rw_fail k = rw_fail.
-  Proof using. reflexivity. Qed.
-
-  Lemma Proper_rw_bind (T U : Type)
-  : Proper (mrw_equiv (@eq T) ==> (pointwise_relation (mrw_equiv (@eq U))) ==>
-            mrw_equiv (@eq U)) (@rw_bind T U).
-  Proof using.
-    red. red. red. red. unfold rw_bind. intros.
-    red in H.
-    specialize (H a b c d e f g).
-    destruct H. constructor.
-    destruct H. subst.
-    eapply H0.
-  Qed.
-
-  Instance Injective_mrw_equiv_rw_ret {T} (rT : T -> T -> Prop) (a b : T)
-  : Injective (mrw_equiv rT (rw_ret a) (rw_ret b)) :=
-  { result := rT a b }.
-  Proof using.
-    unfold rw_ret. intros. red in H.
-    specialize (H nil nil nil 0 0 _ (@TopSubst _ _ nil nil)).
-    inv_all. assumption.
-  Defined.
-  (** End of monad definitions **)
-
-  (* [Progressing T] = [option T] but adds the information that the result
-   * makes progress or does not, i.e. a [Progressing T] is relative to an
-   * input [in]. If the output is [NoProgress] then the meaning is the same as
-   * the input, if the result is [Progress x] then [x] is assumed to be
-   * different than [in].
-   *)
-  Inductive Progressing (T : Type) : Type :=
-  | Progress (new_val : T)
-  | NoProgress.
-
-  Arguments NoProgress {_}.
-
-  Definition ProgressD {T} (a : T) (x : Progressing T) : T :=
-    match x with
-    | Progress x => x
-    | NoProgress => a
-    end.
-
-  Definition fmap_Progressing {T U : Type} (f : T -> U) (x : Progressing T)
-    : Progressing U :=
-    match x with
-    | NoProgress => NoProgress
-    | Progress x => Progress (f x)
-    end.
-
   Local Existing Instance Subst_ctx_subst.
   Local Existing Instance SubstOk_ctx_subst.
   Local Existing Instance SubstUpdate_ctx_subst.
@@ -270,97 +76,13 @@ Section setoid.
   Local Existing Instance Expr_expr.
   Local Existing Instance ExprOk_expr.
 
-  (** These are the core specifications. **)
-  (****************************************)
-
-  (* [setoid_rewrite_rel e r rw] states that if [rw] is run on any context that
-   * [e] is well-typed in, then the final context will extend the initial
-   * context and the result will be related at [r]
-   *)
-  Definition setoid_rewrite_rel
-             (e : expr typ func) (r : R)
-             (rw : mrw (Progressing (expr typ func)))
-  : Prop :=
-    forall (ctx : Ctx typ (expr typ func)) cs (tvs' : tenv typ) cs'
-           (e' : Progressing (expr typ func)),
-      let tus := getUVars ctx in
-      let tvs := getVars ctx in
-      rw tvs' tus tvs (length tus) (length tvs) ctx cs = Some (e', cs') ->
-      WellFormed_ctx_subst cs ->
-      WellFormed_ctx_subst cs' /\
-      forall t rD,
-      RD RbaseD r t = Some rD ->
-      match pctxD cs
-          , lambda_exprD tus (tvs' ++ tvs) t e
-          , pctxD cs'
-          , lambda_exprD tus (tvs' ++ tvs) t (ProgressD e e')
-      with
-      | Some _ , Some eD , Some csD' , Some eD' =>
-        SubstMorphism cs cs' /\
-        (forall (us : HList.hlist typD (getAmbientUVars ctx))
-                (vs : HList.hlist typD (getAmbientVars ctx)),
-            csD' (fun (us : HList.hlist typD (getUVars ctx))
-                      (vs : HList.hlist typD (getVars ctx)) =>
-                    forall vs',
-                      rD (eD us (hlist_app vs' vs))
-                         (eD' us (hlist_app vs' vs))) us vs)
-      | None , _ , _ , _
-      | Some _ , None , _ , _ => True
-      | Some _ , Some _ , None , _
-      | Some _ , Some _ , Some _ , None => False
-      end.
-
-  (* [setoid_rewrite_spec rw] simply states that [rw] is sound for every
-   * [e] and [r].
-   *)
-  Definition setoid_rewrite_spec
-             (rw : expr typ func -> R -> mrw (Progressing (expr typ func)))
-  : Prop :=
-    forall e r, @setoid_rewrite_rel e r (rw e r).
-
-  (* This definition is used for recursive rewriting, it computes a list of
-   * sufficient relations to rewrite in the arguments. It is specialized to
-   * justify termination.
-   *   [respectful_spec resp] states that [resp e r = rs] implies
-   *   [Proper (rs ==> r) e]
-   * TODO(gmalecha):
-   *   This can be generalized a bit to support changing the result argument
-   *)
-  Definition respectful_spec (respectful : expr typ func -> R -> mrw (list R))
-  : Prop :=
-    forall tvs' (ctx : Ctx typ (expr typ func)) cs cs' e r rs,
-      let tus := getUVars ctx in
-      let tvs := getVars ctx in
-      respectful e r tvs' tus tvs (length tus) (length tvs) ctx cs = Some (rs,cs') ->
-      WellFormed_ctx_subst cs ->
-      WellFormed_ctx_subst cs' /\
-      forall ts t rD,
-      RD RbaseD r t = Some rD ->
-      match pctxD cs
-          , lambda_exprD tus (tvs' ++ tvs) (fold_right (typ2 (F:=RFun)) t ts) e
-          , pctxD cs'
-          , RD RbaseD (fold_right Rrespects r rs) (fold_right (typ2 (F:=RFun)) t ts)
-      with
-      | Some _ , Some eD , Some csD' , Some rD' =>
-        SubstMorphism cs cs' /\
-        (forall (us : HList.hlist typD (getAmbientUVars ctx))
-                (vs : HList.hlist typD (getAmbientVars ctx)),
-            csD' (fun (us : HList.hlist typD (getUVars ctx))
-                      (vs : HList.hlist typD (getVars ctx)) =>
-                    forall vs',
-                      Proper rD' (eD us (hlist_app vs' vs))) us vs)
-      | None , _ , _ , _
-      | Some _ , None , _ , _ => True
-      | Some _ , Some _ , None , _
-      | Some _ , Some _ , Some _ , None => False
-      end.
 
   (** This is the core of the rewriter which applies respectful and performs
    ** recursive rewriting.
    **)
   Section setoid_rewrite.
     Definition arg_rewriter : Type :=
-      expr typ func * (R -> mrw (Progressing (expr typ func))).
+      expr typ func * (R -> mrw typ func (Progressing (expr typ func))).
 
     (* This structure is similar in spirit to hereditary substitutions where
      * arguments are paired with the functions used to rewrite them. This allows
@@ -370,15 +92,15 @@ Section setoid.
     : expr typ func ->
       forall (es : list arg_rewriter)
              (rg : R),
-        mrw (Progressing (expr typ func)).
+        mrw typ func (Progressing (expr typ func)).
 
     (* This is the core rewriter.
      *   [setoid_rewrite' e es r] performs rewriting on [e @ es] with respect
      *   to relation [r].
      *)
-    Fixpoint setoid_rewrite'
+    Local Fixpoint setoid_rewrite'
              (e : expr typ func) (es : list arg_rewriter) (rg : R)
-    : mrw (Progressing (expr typ func)) :=
+    : mrw typ func (Progressing (expr typ func)) :=
       match e with
       | App f x =>
         setoid_rewrite' f ((x, setoid_rewrite' x nil) :: es) rg
@@ -405,26 +127,26 @@ Section setoid.
       end.
 
     Definition setoid_rewrite (e : expr typ func) (rg : R)
-    : mrw (Progressing (expr typ func)) :=
+    : mrw typ func (Progressing (expr typ func)) :=
       setoid_rewrite' e nil rg.
 
-    Definition setoid_rewrite_rec (ls : list arg_rewriter)
+    Local Definition setoid_rewrite_rec (ls : list arg_rewriter)
     : Prop :=
       Forall (fun e =>
                 forall r,
-                  @setoid_rewrite_rel (fst e) r (snd e r)) ls.
+                  setoid_rewrite_rel RbaseD (fst e) r (snd e r)) ls.
 
     Hypothesis respectfulness_sound
     : forall e es rg,
-        @setoid_rewrite_rec es ->
-        @setoid_rewrite_rel (apps e (map fst es))
-                            rg (respectfulness e es rg).
+        setoid_rewrite_rec es ->
+        setoid_rewrite_rel RbaseD (apps e (map fst es))
+                           rg (respectfulness e es rg).
 
-    Lemma setoid_rewrite'_sound
+    Local Lemma setoid_rewrite'_sound
     : forall e es rg,
-        @setoid_rewrite_rec es ->
-        @setoid_rewrite_rel (apps e (map fst es))
-                            rg (setoid_rewrite' e es rg).
+        setoid_rewrite_rec es ->
+        setoid_rewrite_rel RbaseD (apps e (map fst es))
+                           rg (setoid_rewrite' e es rg).
     Proof using RSymOk_func RTypeOk_typD Typ2Ok_Fun respectfulness_sound.
       induction e; eauto using respectfulness_sound.
       { simpl in *. intros.
@@ -501,7 +223,7 @@ Section setoid.
 
     Theorem setoid_rewrite_sound
     : forall e rg,
-        @setoid_rewrite_rel e rg (setoid_rewrite e rg).
+        setoid_rewrite_rel RbaseD e rg (setoid_rewrite e rg).
     Proof using RSymOk_func RTypeOk_typD Typ2Ok_Fun respectfulness_sound.
       intros. eapply setoid_rewrite'_sound.
       constructor.
@@ -512,14 +234,14 @@ Section setoid.
   Section top_bottom.
     Context (reflexive : refl_dec R)
             (transitive : trans_dec R)
-            (rw : expr typ func -> R -> mrw (Progressing (expr typ func)))
-            (respectful : expr typ func -> R -> mrw (list R)).
+            (rw : expr typ func -> R -> @mrw typ func (Progressing (expr typ func)))
+            (respectful : expr typ func -> R -> @mrw typ func (list R)).
 
     Hypothesis reflexiveOk : refl_dec_ok (RD RbaseD) reflexive.
     Hypothesis transitiveOk : trans_dec_ok (RD RbaseD) transitive.
 
-    Hypothesis rwOk : setoid_rewrite_spec rw.
-    Hypothesis respectfulOk : respectful_spec respectful.
+    Hypothesis rwOk : setoid_rewrite_spec RbaseD rw.
+    Hypothesis respectfulOk : respectful_spec RbaseD respectful.
 
     (** TODO(gmalecha): Move **)
     Lemma lambda_exprD_App
@@ -560,10 +282,10 @@ Section setoid.
       { rewrite H0 in H. congruence. }
     Qed.
 
-    Fixpoint recursive_rewrite' (prog : bool) (f : expr typ func)
+    Local Fixpoint recursive_rewrite' (prog : bool) (f : expr typ func)
              (es : list arg_rewriter)
              (rs : list R)
-    : mrw (Progressing (expr typ func)) :=
+    : mrw typ func (Progressing (expr typ func)) :=
       match es , rs with
       | nil , nil => rw_ret (if prog then Progress f else NoProgress)
       | (e,rec) :: es , r :: rs =>
@@ -849,7 +571,7 @@ Section setoid.
      ** the possibility of redundant back-tracking?
      **)
     Definition bottom_up (e : expr typ func) (r : R)
-    : mrw (Progressing (expr typ func)) :=
+    : mrw typ func (Progressing (expr typ func)) :=
       setoid_rewrite
         (fun e efs r =>
 	   let es := map fst efs in
@@ -928,7 +650,7 @@ Section setoid.
 
     Lemma bottom_up_sound_lem
     : forall e rg,
-        @setoid_rewrite_rel e rg (bottom_up e rg).
+        setoid_rewrite_rel RbaseD e rg (bottom_up e rg).
     Proof using RSymOk_func RTypeOk_typD RbaseD_single_type Typ2Ok_Fun
           reflexiveOk respectfulOk rwOk transitiveOk.
       unfold bottom_up. intros.
@@ -1166,7 +888,7 @@ Section setoid.
     Time Qed.
 
     Theorem bottom_up_sound
-    : setoid_rewrite_spec bottom_up.
+    : setoid_rewrite_spec RbaseD bottom_up.
     Proof using RSymOk_func RTypeOk_typD RbaseD_single_type Typ2Ok_Fun
           reflexiveOk respectfulOk rwOk transitiveOk.
       intros. red. eapply bottom_up_sound_lem.
@@ -1200,110 +922,4 @@ Section setoid.
 *)
   End top_bottom.
 
-
-  (** This should probably go somewhere else **)
-  Section the_tactic.
-
-    Definition lem_rewriter : Type :=
-      expr typ func -> R -> mrw (Progressing (expr typ func)).
-    Definition respectful_dec : Type :=
-      expr typ func -> R -> mrw (list R).
-
-  Definition auto_setoid_rewrite_bu
-             (r : R)
-             (reflexive : refl_dec R)
-             (transitive : trans_dec R)
-             (rewriter : lem_rewriter)
-             (respectful : respectful_dec)
-  : rtac typ (expr typ func) :=
-    let rw := bottom_up reflexive transitive rewriter respectful in
-    fun tus tvs nus nvs ctx cs g =>
-      match @rw g r nil tus tvs nus nvs ctx cs with
-      | None => Fail
-      | Some (Progress g', cs') => More_ cs' (GGoal g')
-      | Some (NoProgress, cs') => Fail
-      end.
-
-  Variable R_impl : R.
-
-  Hypothesis R_impl_is_impl
-    : RD RbaseD R_impl (typ0 (F:=Prop)) =
-      Some match eq_sym (typ0_cast (F:=Prop)) in _ = t return t -> t -> Prop with
-           | eq_refl => Basics.impl
-           end.
-
-  Theorem auto_setoid_rewrite_bu_sound
-  : forall is_refl is_trans rw proper
-           (His_reflOk : refl_dec_ok (RD RbaseD) is_refl)
-           (His_transOk : trans_dec_ok (RD RbaseD) is_trans),
-      setoid_rewrite_spec rw ->
-      respectful_spec proper ->
-      rtac_sound (auto_setoid_rewrite_bu (Rflip R_impl)
-                                         is_refl is_trans rw proper).
-  Proof using RSymOk_func RTypeOk_typD R_impl_is_impl
-        RbaseD_single_type Typ2Ok_Fun.
-    intros. unfold auto_setoid_rewrite_bu. red.
-    intros.
-    generalize (@bottom_up_sound is_refl is_trans rw proper
-                                 His_reflOk His_transOk H H0 g (Rflip R_impl) ctx s nil).
-    simpl.
-    destruct (bottom_up is_refl is_trans rw proper g (Rflip R_impl) nil
-      (getUVars ctx) (getVars ctx) (length (getUVars ctx))
-      (length (getVars ctx)) s).
-    { destruct p. destruct p; subst; eauto using rtac_spec_Fail.
-      red. intros Hbus ? ?.
-      specialize (Hbus _ _ eq_refl H2).
-      forward_reason.
-      split; try assumption.
-      split; [ constructor | ].
-      specialize (H4 (typ0 (F:=Prop))).
-      rewrite R_impl_is_impl in H4.
-      specialize (H4 _ eq_refl).
-      revert H4.
-      destruct (pctxD s) eqn:HpctxDs; try (clear; tauto).
-      simpl. unfold propD. unfold exprD_typ0.
-      simpl.
-      destruct (lambda_exprD (getUVars ctx) (getVars ctx) (typ0 (F:=Prop)) g);
-        try solve [ tauto ].
-      destruct (pctxD c) eqn:HpctxDc; try solve [ tauto ].
-      destruct (lambda_exprD (getUVars ctx) (getVars ctx) (typ0 (F:=Prop)) new_val);
-        try solve [ tauto ].
-      destruct 1; split; try assumption.
-      intros.
-      gather_facts.
-      eapply Pure_pctxD; eauto.
-      intros.
-      specialize (H5 Hnil). simpl in *.
-      revert H6 H5. autorewrite_with_eq_rw.
-      clear. generalize (typ0_cast (F:=Prop)).
-      generalize dependent (typD (typ0 (F:=Prop))).
-      do 4 intro. subst. simpl.
-      unfold flip, Basics.impl. tauto. }
-    { subst. intro. clear.
-      eapply rtac_spec_Fail. }
-  Qed.
-
-  End the_tactic.
-
 End setoid.
-
-(* This fast-path eliminates the need to build environments when
- * unification is definitely going to fail
-    Fixpoint checkUnify (e1 e2 : expr typ func) : bool :=
-      match e1 , e2 with
-      | ExprCore.UVar _ , _ => true
-      | ExprCore.Var v1 , ExprCore.Var v2 => v1 ?[ eq ] v2
-      | Inj a , Inj b => a ?[ eq ] b
-      | App f1 x1 , App f2 x2 => checkUnify f1 f2
-      | Abs _ _ , Abs _ _ => true
-      | _ , ExprCore.UVar _ => true
-      | _ , _ => false
-      end.
- *)
-
-Arguments NoProgress {_}.
-Arguments Progress {_} _.
-Arguments lem_rewriter typ func Rbase : clear implicits.
-Arguments respectful_dec typ func Rbase : clear implicits.
-
-Export MirrorCore.Lambda.RewriteRelations.
