theories/Lambda/Polymorphic.v
@@ -1,0 +1,23 @@
+Require Import ExtLib.Data.Vector.
+
+Set Implicit Arguments.
+Set Strict Implicit.
+
+Section poly.
+  Variable typ : Type.
+
+  Fixpoint polymorphic (n : nat) T : Type :=
+    match n with
+    | 0 => T
+    | S n => typ -> polymorphic n T
+    end.
+
+  Fixpoint inst {T} (n : nat)
+  : polymorphic n T -> vector typ n -> T :=
+    match n as n return polymorphic n T -> vector typ n -> T with
+    | 0 => fun p _ => p
+    | S n => fun p a => inst (p (Vector.vector_hd a)) (Vector.vector_tl a)
+    end.
+End poly.
+
+Arguments inst {typ T n} p v : clear implicits, rename.
