theories/Lambda/Rewrite/Core.v
@@ -1,0 +1,384 @@
+Require Import Coq.omega.Omega.
+Require Import Coq.Classes.Morphisms.
+Require Import Coq.PArith.BinPos.
+Require Import Coq.Relations.Relations.
+Require Import Coq.FSets.FMapPositive.
+Require Import ExtLib.Core.RelDec.
+Require Import ExtLib.Data.Positive.
+Require Import ExtLib.Data.List.
+Require Import ExtLib.Data.HList.
+Require Import ExtLib.Data.Option.
+Require Import ExtLib.Data.Pair.
+Require Import ExtLib.Recur.Relation.
+Require Import ExtLib.Recur.GenRec.
+Require Import ExtLib.Recur.Facts.
+Require Import ExtLib.Tactics.
+Require Import MirrorCore.SubstI.
+Require Import MirrorCore.Lemma.
+Require Import MirrorCore.VarsToUVars.
+Require Import MirrorCore.Instantiate.
+Require Import MirrorCore.Util.Forwardy.
+Require Import MirrorCore.Util.Compat.
+Require Import MirrorCore.Util.Iteration.
+Require Import MirrorCore.RTac.Core.
+Require Import MirrorCore.Lambda.Expr.
+Require Import MirrorCore.Lambda.ExprTac.
+Require Import MirrorCore.Lambda.ExprUnify.
+Require Import MirrorCore.Lambda.AppN.
+Require Import MirrorCore.Lambda.ExprSubstitute.
+Require Import MirrorCore.Lambda.RewriteRelations.
+
+Set Implicit Arguments.
+Set Strict Implicit.
+
+Set Suggest Proof Using.
+
+Section setoid.
+  Context {typ : Type}.
+  Context {func : Type}.
+  Context {RType_typD : RType typ}.
+  Context {Typ2_Fun : Typ2 RType_typD RFun}.
+  Context {RSym_func : RSym func}.
+
+  (** Reasoning principles **)
+  Context {RTypeOk_typD : RTypeOk}.
+  Context {Typ2Ok_Fun : Typ2Ok Typ2_Fun}.
+  Context {RSymOk_func : RSymOk RSym_func}.
+  Context {Typ0_Prop : Typ0 _ Prop}.
+
+  (** TODO(gmalecha): This is not necessary *)
+  Context {RelDec_eq_typ : RelDec (@eq typ)}.
+  Context {RelDec_Correct_eq_typ : RelDec_Correct RelDec_eq_typ}.
+
+  (* TODO(gmalecha): Wrap all of this up in a type class?
+   * Why should it be different than Expr?
+   *)
+  Variable Rbase : Type.
+  Variable Rbase_eq : Rbase -> Rbase -> bool.
+  Hypothesis Rbase_eq_ok : forall a b, Rbase_eq a b = true -> a = b.
+
+  Local Notation "'R'" := (R typ Rbase).
+
+  Variable RbaseD : Rbase -> forall t : typ, option (typD t -> typD t -> Prop).
+
+  Hypothesis RbaseD_single_type
+  : forall r t1 t2 rD1 rD2,
+      RbaseD r t1 = Some rD1 ->
+      RbaseD r t2 = Some rD2 ->
+      t1 = t2.
+
+
+  (** This monad abstracts the idea of working under a context.
+   ** It is morally exactly the same as [rtac] except for two differences:
+   ** 1) It is generalized over the goal representation so it can avoid
+   **    manifesting [Goal]s
+   ** 2) It has an extra [tvs'] argument that allows it to avoid pushing
+   **    terms into the context when it does not need to.
+   **
+   ** TODO(gmalecha):
+   **   This should be unified with the [rtac] monad but understanding
+   **   the full design still requires a bit more work.
+   **)
+  Definition mrw (T : Type) : Type :=
+    tenv typ -> tenv typ -> tenv typ -> nat -> nat ->
+    forall c : Ctx typ (expr typ func), ctx_subst c ->
+                                        option (T * ctx_subst c).
+
+  Definition rw_ret {T} (val : T) : mrw T :=
+    fun _ _ _ _ _ _ s => Some (val, s).
+
+  Definition rw_bind {T U} (c : mrw T) (k : T -> mrw U) : mrw U :=
+    fun tvs' tus tvs nus nvs ctx cs =>
+      match c tvs' tus tvs nus nvs ctx cs with
+      | None => None
+      | Some (v,cs') => k v tvs' tus tvs nus nvs ctx cs'
+      end.
+
+  Definition rw_orelse {T} (c1 c2 : mrw T) : mrw T :=
+    fun tvs' tus tvs nus nvs ctx cs =>
+      match c1 tvs' tus tvs nus nvs ctx cs with
+      | None => c2 tvs' tus tvs nus nvs ctx cs
+      | z => z
+      end.
+
+  Definition rw_fail {T} : mrw T :=
+    fun tvs' tus tvs nus nvs ctx cs =>
+      None.
+
+  Definition rw_bind_catch {T U : Type} (c : mrw T) (k : T -> mrw U)
+             (otherwise : mrw U)
+  : mrw U :=
+    fun tus' tus tvs nus nvs ctx cs =>
+      match c tus' tus tvs nus nvs ctx cs with
+      | None => otherwise tus' tus tvs nus nvs ctx cs
+      | Some (val,cs') => k val tus' tus tvs nus nvs ctx cs'
+      end.
+
+  Lemma rw_orelse_case
+  : forall (T : Type) (A B : mrw T) a b c d e f g h,
+      @rw_orelse _ A B a b c d e f g = h ->
+      A a b c d e f g = h \/
+      B a b c d e f g = h.
+  Proof using.
+    unfold rw_orelse. intros.
+    forward.
+  Qed.
+
+  Lemma rw_bind_catch_case
+  : forall (T U : Type) (A : mrw T) (B : T -> mrw U) (C : mrw U)
+           a b c d e f g h,
+      @rw_bind_catch _ _ A B C a b c d e f g = h ->
+      (exists x g', A a b c d e f g = Some (x,g') /\
+                    B x a b c d e f g' = h) \/
+      (C a b c d e f g = h /\ A a b c d e f g = None).
+  Proof using.
+    unfold rw_bind_catch. intros; forward.
+    left. do 2 eexists; split; eauto.
+  Qed.
+
+  Lemma rw_bind_case
+  : forall (T U : Type) (A : mrw T) (B : T -> mrw U)
+           a b c d e f g h,
+      @rw_bind _ _ A B a b c d e f g = Some h ->
+      exists x g',
+        A a b c d e f g = Some (x, g') /\
+        B x a b c d e f g' = Some h.
+  Proof using.
+    unfold rw_bind. intros; forward.
+    do 2 eexists; eauto.
+  Qed.
+
+  Section rw_map2.
+    Context {T U V : Type}.
+    Variable f : T -> U -> mrw V.
+
+    Fixpoint rw_map2 (ts : list T) (us : list U) : mrw (list V) :=
+      match ts , us with
+        | nil , nil => rw_ret nil
+        | t :: ts , u :: us =>
+          rw_bind (f t u) (fun v =>
+                             rw_bind (rw_map2 ts us)
+                                     (fun vs => rw_ret (v :: vs)))
+        | _ , _ => rw_fail
+      end.
+  End rw_map2.
+
+  Definition mrw_equiv {T} (rT : T -> T -> Prop) (l : mrw T) (r : mrw T)
+  : Prop :=
+    forall a b c d e f g,
+      Roption (Eqpair rT eq) (l a b c d e f g) (r a b c d e f g).
+
+  Instance Reflexive_mrw_equiv {T} (rT : T -> T -> Prop)
+           {Refl_rT : Reflexive rT}
+  : Reflexive (mrw_equiv rT).
+  Proof using.
+    red. red. intros. eapply Reflexive_Roption. eapply Reflexive_Eqpair; eauto.
+  Qed.
+
+  Instance Symmetric_mrw_equiv {T} (rT : T -> T -> Prop)
+           {Sym_rT : Symmetric rT}
+  : Symmetric (mrw_equiv rT).
+  Proof using.
+    red. red. intros. eapply Symmetric_Roption. eapply Symmetric_Eqpair; eauto.
+    eapply H.
+  Qed.
+
+  Instance Transitive_mrw_equiv {T} (rT : T -> T -> Prop)
+           {Trans_rT : Transitive rT}
+  : Transitive (mrw_equiv rT).
+  Proof using.
+    red. red. intros. eapply Transitive_Roption.
+    eapply Transitive_Eqpair; eauto with typeclass_instances.
+    eapply H. eapply H0.
+  Qed.
+
+  Lemma rw_bind_assoc
+  : forall {T U V} (c : mrw T) (k : T -> mrw U) (k' : U -> mrw V),
+      mrw_equiv eq
+                (rw_bind (rw_bind c k) k')
+                (rw_bind c (fun x => rw_bind (k x) k')).
+  Proof using.
+    unfold rw_bind. simpl.
+    red. intros.
+    destruct (c a b c0 d e f g); try constructor.
+    destruct p.
+    eapply Reflexive_Roption. apply Reflexive_Eqpair; eauto.
+  Qed.
+
+  Lemma rw_bind_rw_ret
+  : forall {T U} (x : T) (k : T -> mrw U),
+      rw_bind (rw_ret x) k = k x.
+  Proof using. reflexivity. Qed.
+
+  Lemma rw_bind_rw_fail
+  : forall {T U} (k : T -> mrw U),
+      rw_bind rw_fail k = rw_fail.
+  Proof using. reflexivity. Qed.
+
+  Lemma Proper_rw_bind (T U : Type)
+  : Proper (mrw_equiv (@eq T) ==> (pointwise_relation (mrw_equiv (@eq U))) ==>
+            mrw_equiv (@eq U)) (@rw_bind T U).
+  Proof using.
+    red. red. red. red. unfold rw_bind. intros.
+    red in H.
+    specialize (H a b c d e f g).
+    destruct H. constructor.
+    destruct H. subst.
+    eapply H0.
+  Qed.
+
+  Instance Injective_mrw_equiv_rw_ret {T} (rT : T -> T -> Prop) (a b : T)
+  : Injective (mrw_equiv rT (rw_ret a) (rw_ret b)) :=
+  { result := rT a b }.
+  Proof using.
+    unfold rw_ret. intros. red in H.
+    specialize (H nil nil nil 0 0 _ (@TopSubst _ _ nil nil)).
+    inv_all. assumption.
+  Defined.
+  (** End of monad definitions **)
+
+  (* [Progressing T] = [option T] but adds the information that the result
+   * makes progress or does not, i.e. a [Progressing T] is relative to an
+   * input [in]. If the output is [NoProgress] then the meaning is the same as
+   * the input, if the result is [Progress x] then [x] is assumed to be
+   * different than [in].
+   *)
+  Inductive Progressing (T : Type) : Type :=
+  | Progress (new_val : T)
+  | NoProgress.
+
+  Arguments NoProgress {_}.
+
+  Definition ProgressD {T} (a : T) (x : Progressing T) : T :=
+    match x with
+    | Progress x => x
+    | NoProgress => a
+    end.
+
+  Definition fmap_Progressing {T U : Type} (f : T -> U) (x : Progressing T)
+    : Progressing U :=
+    match x with
+    | NoProgress => NoProgress
+    | Progress x => Progress (f x)
+    end.
+
+  Local Existing Instance Subst_ctx_subst.
+  Local Existing Instance SubstOk_ctx_subst.
+  Local Existing Instance SubstUpdate_ctx_subst.
+  Local Existing Instance SubstUpdateOk_ctx_subst.
+  Local Existing Instance Expr_expr.
+  Local Existing Instance ExprOk_expr.
+
+  (** These are the core specifications. **)
+  (****************************************)
+
+  (* [setoid_rewrite_rel e r rw] states that if [rw] is run on any context that
+   * [e] is well-typed in, then the final context will extend the initial
+   * context and the result will be related at [r]
+   *)
+  Definition setoid_rewrite_rel
+             (e : expr typ func) (r : R)
+             (rw : mrw (Progressing (expr typ func)))
+  : Prop :=
+    forall (ctx : Ctx typ (expr typ func)) cs (tvs' : tenv typ) cs'
+           (e' : Progressing (expr typ func)),
+      let tus := getUVars ctx in
+      let tvs := getVars ctx in
+      rw tvs' tus tvs (length tus) (length tvs) ctx cs = Some (e', cs') ->
+      WellFormed_ctx_subst cs ->
+      WellFormed_ctx_subst cs' /\
+      forall t rD,
+      RD RbaseD r t = Some rD ->
+      match pctxD cs
+          , lambda_exprD tus (tvs' ++ tvs) t e
+          , pctxD cs'
+          , lambda_exprD tus (tvs' ++ tvs) t (ProgressD e e')
+      with
+      | Some _ , Some eD , Some csD' , Some eD' =>
+        SubstMorphism cs cs' /\
+        (forall (us : HList.hlist typD (getAmbientUVars ctx))
+                (vs : HList.hlist typD (getAmbientVars ctx)),
+            csD' (fun (us : HList.hlist typD (getUVars ctx))
+                      (vs : HList.hlist typD (getVars ctx)) =>
+                    forall vs',
+                      rD (eD us (hlist_app vs' vs))
+                         (eD' us (hlist_app vs' vs))) us vs)
+      | None , _ , _ , _
+      | Some _ , None , _ , _ => True
+      | Some _ , Some _ , None , _
+      | Some _ , Some _ , Some _ , None => False
+      end.
+
+  (* [setoid_rewrite_spec rw] simply states that [rw] is sound for every
+   * [e] and [r].
+   *)
+  Definition setoid_rewrite_spec
+             (rw : expr typ func -> R -> mrw (Progressing (expr typ func)))
+  : Prop :=
+    forall e r, @setoid_rewrite_rel e r (rw e r).
+
+  (* This definition is used for recursive rewriting, it computes a list of
+   * sufficient relations to rewrite in the arguments. It is specialized to
+   * justify termination.
+   *   [respectful_spec resp] states that [resp e r = rs] implies
+   *   [Proper (rs ==> r) e]
+   * TODO(gmalecha):
+   *   This can be generalized a bit to support changing the result argument
+   *)
+  Definition respectful_spec (respectful : expr typ func -> R -> mrw (list R))
+  : Prop :=
+    forall tvs' (ctx : Ctx typ (expr typ func)) cs cs' e r rs,
+      let tus := getUVars ctx in
+      let tvs := getVars ctx in
+      respectful e r tvs' tus tvs (length tus) (length tvs) ctx cs = Some (rs,cs') ->
+      WellFormed_ctx_subst cs ->
+      WellFormed_ctx_subst cs' /\
+      forall ts t rD,
+      RD RbaseD r t = Some rD ->
+      match pctxD cs
+          , lambda_exprD tus (tvs' ++ tvs) (fold_right (typ2 (F:=RFun)) t ts) e
+          , pctxD cs'
+          , RD RbaseD (fold_right Rrespects r rs) (fold_right (typ2 (F:=RFun)) t ts)
+      with
+      | Some _ , Some eD , Some csD' , Some rD' =>
+        SubstMorphism cs cs' /\
+        (forall (us : HList.hlist typD (getAmbientUVars ctx))
+                (vs : HList.hlist typD (getAmbientVars ctx)),
+            csD' (fun (us : HList.hlist typD (getUVars ctx))
+                      (vs : HList.hlist typD (getVars ctx)) =>
+                    forall vs',
+                      Proper rD' (eD us (hlist_app vs' vs))) us vs)
+      | None , _ , _ , _
+      | Some _ , None , _ , _ => True
+      | Some _ , Some _ , None , _
+      | Some _ , Some _ , Some _ , None => False
+      end.
+
+  Definition lem_rewriter : Type :=
+    expr typ func -> R -> mrw (Progressing (expr typ func)).
+  Definition respectful_dec : Type :=
+    expr typ func -> R -> mrw (list R).
+
+End setoid.
+
+(* This fast-path eliminates the need to build environments when
+ * unification is definitely going to fail
+    Fixpoint checkUnify (e1 e2 : expr typ func) : bool :=
+      match e1 , e2 with
+      | ExprCore.UVar _ , _ => true
+      | ExprCore.Var v1 , ExprCore.Var v2 => v1 ?[ eq ] v2
+      | Inj a , Inj b => a ?[ eq ] b
+      | App f1 x1 , App f2 x2 => checkUnify f1 f2
+      | Abs _ _ , Abs _ _ => true
+      | _ , ExprCore.UVar _ => true
+      | _ , _ => false
+      end.
+ *)
+
+Arguments mrw _ _ _ : clear implicits.
+Arguments NoProgress {_}.
+Arguments Progress {_} _.
+Arguments lem_rewriter typ func Rbase : clear implicits.
+Arguments respectful_dec typ func Rbase : clear implicits.
+
+Export MirrorCore.Lambda.RewriteRelations.
