theories/Lambda/Rewrite/HintDbs.v
@@ -1,0 +1,145 @@
+Require Import Coq.omega.Omega.
+Require Import Coq.Classes.Morphisms.
+Require Import Coq.PArith.BinPos.
+Require Import Coq.Relations.Relations.
+Require Import Coq.FSets.FMapPositive.
+Require Import ExtLib.Core.RelDec.
+Require Import ExtLib.Data.Positive.
+Require Import ExtLib.Tactics.
+Require Import MirrorCore.SubstI.
+Require Import MirrorCore.Lemma.
+Require Import MirrorCore.VarsToUVars.
+Require Import MirrorCore.Instantiate.
+Require Import MirrorCore.Util.Forwardy.
+Require Import MirrorCore.Util.Compat.
+Require Import MirrorCore.Util.Iteration.
+Require Import MirrorCore.RTac.Core.
+Require Import MirrorCore.RTac.CoreK.
+Require Import MirrorCore.Lambda.Expr.
+Require Import MirrorCore.Lambda.ExprTac.
+Require Import MirrorCore.Lambda.ExprUnify.
+Require Import MirrorCore.Lambda.AppN.
+Require Import MirrorCore.Lambda.ExprSubstitute.
+Require Import MirrorCore.Lambda.RewriteRelations.
+Require Import MirrorCore.Lambda.Rewrite.Core.
+Require Import MirrorCore.Lambda.Polymorphic.
+Require Import MirrorCore.Lambda.PolyInst.
+Require Import MirrorCore.Views.View.
+Require Import MirrorCore.MTypes.ModularTypes.
+Require Import MirrorCore.MTypes.MTypeUnify.
+
+Set Implicit Arguments.
+Set Strict Implicit.
+
+Set Suggest Proof Using.
+
+Section setoid.
+  Context {tsym : nat -> Type}.
+  Let typ := mtyp tsym.
+  Context {func : Type}.
+  Context {RType_typD : RType typ}.
+  Context {Typ2_Fun : Typ2 RType_typD RFun}.
+  Context {RSym_func : RSym func}.
+
+  (** Reasoning principles **)
+  Context {RTypeOk_typD : RTypeOk}.
+  Context {Typ2Ok_Fun : Typ2Ok Typ2_Fun}.
+  Context {RSymOk_func : RSymOk RSym_func}.
+  Context {Typ0_Prop : Typ0 _ Prop}.
+
+  Local Existing Instance Subst_ctx_subst.
+  Local Existing Instance SubstOk_ctx_subst.
+  Local Existing Instance SubstUpdate_ctx_subst.
+  Local Existing Instance SubstUpdateOk_ctx_subst.
+  Local Existing Instance Expr_expr.
+  Local Existing Instance ExprOk_expr.
+
+  (* TODO(gmalecha): Wrap all of this up in a type class?
+   * Why should it be different than Expr?
+   *)
+  Variable Rbase : Type.
+  Variable Rbase_eq : Rbase -> Rbase -> bool.
+  Hypothesis Rbase_eq_ok : forall a b, Rbase_eq a b = true -> a = b.
+
+  Local Notation "'R'" := (R typ Rbase).
+
+  Variable RbaseD : Rbase -> forall t : typ, option (typD t -> typD t -> Prop).
+
+  Hypothesis RbaseD_single_type
+  : forall r t1 t2 rD1 rD2,
+      RbaseD r t1 = Some rD1 ->
+      RbaseD r t2 = Some rD2 ->
+      t1 = t2.
+
+  Fixpoint polymorphic (n : nat) T : Type :=
+    match n with
+    | 0 => T
+    | S n => typ -> polymorphic n T
+    end.
+
+  Inductive HintRewrite : Type :=
+  | PRw : forall n,
+      polymorphic n (rw_lemma typ func Rbase) ->
+      rtacK typ (expr typ func) ->
+      HintRewrite
+  | Rw : rw_lemma typ func Rbase -> rtacK typ (expr typ func) ->
+         HintRewrite.
+
+  Definition RewriteHintDb : Type :=
+    list HintRewrite.
+
+  Context {PV_vtype : PartialView (tsym 0) VType}.
+
+  Section fmap_polymorphic.
+    Variables T U : Type.
+    Variable f : T -> U.
+    Fixpoint fmap_polymorphic (n : nat)
+    : polymorphic n T -> polymorphic n U :=
+      match n with
+      | 0 => f
+      | S n => fun x y => fmap_polymorphic n (x y)
+      end.
+  End fmap_polymorphic.
+
+  Require Import ExtLib.Structures.Functor.
+  Instance Functor_polymorphic n : Functor (polymorphic n) :=
+  { fmap := fun T U f => @fmap_polymorphic T U f n }.
+
+  Local Definition base_update (l : tsym 0) (r : typ) p :=
+    match f_view l with
+    | POption.pNone => Some p
+    | POption.pSome (tVar n) => PolyInst.type_remember n r p
+    end.
+
+  Local Definition view_update :=
+    (mtype_unify tsym (FMapPositive.pmap typ) base_update).
+
+  Let local_view : PartialView typ VType :=
+    PartialView_trans TypeView_sym0 PV_vtype.
+  Local Existing Instance local_view.
+
+  Local Definition get_lemma {n : nat}
+        (p : polymorphic n (rw_lemma typ func Rbase))
+        (e : expr typ func)
+  : option (rw_lemma typ func Rbase) :=
+    match get_inst view_update (fmap (fun x => x.(concl).(lhs)) p) e with
+    | None => None
+    | Some args => Some (inst p args)
+    end.
+
+  Fixpoint CompileHints (hints : RewriteHintDb)
+           (e : expr typ func)
+           (r : R)
+  : list (rw_lemma typ func Rbase * rtacK typ (expr typ func)) :=
+    match hints with
+    | nil => nil
+    | Rw lem tac :: hints =>
+      (lem, tac) :: CompileHints hints e r
+    | PRw n plem tac :: hints =>
+      match get_lemma plem e with
+      | None => CompileHints hints e r
+      | Some lem => (lem, tac) :: CompileHints hints e r
+      end
+    end.
+
+End setoid.
