theories/Lambda/Rewrite/Reduce.v
@@ -1,0 +1,129 @@
+Require Import Coq.Classes.Morphisms.
+Require Import Coq.Relations.Relations.
+Require Import ExtLib.Core.RelDec.
+Require Import ExtLib.Tactics.
+Require Import MirrorCore.Util.Forwardy.
+Require Import MirrorCore.Util.Compat.
+Require Import MirrorCore.Util.Iteration.
+Require Import MirrorCore.Lambda.Expr.
+Require Import MirrorCore.Lambda.ExprTac.
+Require Import MirrorCore.Lambda.ExprSubstitute.
+Require Import MirrorCore.Lambda.RewriteRelations.
+Require Import MirrorCore.Lambda.Rewrite.Core.
+
+Set Implicit Arguments.
+Set Strict Implicit.
+
+Set Suggest Proof Using.
+
+Section setoid.
+  Context {typ : Type}.
+  Context {func : Type}.
+  Context {RType_typD : RType typ}.
+  Context {Typ2_Fun : Typ2 RType_typD RFun}.
+  Context {RSym_func : RSym func}.
+
+  (** Reasoning principles **)
+  Context {RTypeOk_typD : RTypeOk}.
+  Context {Typ2Ok_Fun : Typ2Ok Typ2_Fun}.
+  Context {RSymOk_func : RSymOk RSym_func}.
+  Context {Typ0_Prop : Typ0 _ Prop}.
+
+  (** TODO(gmalecha): This is not necessary *)
+  Context {RelDec_eq_typ : RelDec (@eq typ)}.
+  Context {RelDec_Correct_eq_typ : RelDec_Correct RelDec_eq_typ}.
+
+  Local Existing Instance Subst_ctx_subst.
+  Local Existing Instance SubstOk_ctx_subst.
+  Local Existing Instance SubstUpdate_ctx_subst.
+  Local Existing Instance SubstUpdateOk_ctx_subst.
+  Local Existing Instance Expr_expr.
+  Local Existing Instance ExprOk_expr.
+
+  (* TODO(gmalecha): Wrap all of this up in a type class?
+   * Why should it be different than Expr?
+   *)
+  Variable Rbase : Type.
+  Variable Rbase_eq : Rbase -> Rbase -> bool.
+  Hypothesis Rbase_eq_ok : forall a b, Rbase_eq a b = true -> a = b.
+
+  Local Notation "'R'" := (R typ Rbase).
+
+  Variable RbaseD : Rbase -> forall t : typ, option (typD t -> typD t -> Prop).
+
+  Variable reducer : expr typ func -> expr typ func.
+  Variable lr : lem_rewriter typ func Rbase.
+
+  Definition rw_simplify : lem_rewriter _ _ _ :=
+    fun e => lr (reducer e).
+
+  Hypothesis reducer_sound
+  : forall tus tvs t e eD,
+      lambda_exprD tus tvs t e = Some eD ->
+      exists eD',
+        lambda_exprD tus tvs t (reducer e) = Some eD' /\
+        forall us vs, eD us vs = eD' us vs.
+  Hypothesis lr_sound : setoid_rewrite_spec RbaseD lr.
+
+  Theorem rw_simplify_sound
+  : setoid_rewrite_spec RbaseD rw_simplify.
+  Proof using lr_sound reducer_sound.
+    unfold rw_simplify. do 2 red. intros.
+    eapply lr_sound in H; eauto.
+    forward_reason; split; eauto.
+    intros. eapply H1 in H2; clear H1.
+    forward.
+    specialize (@reducer_sound _ _ _ _ _ H3).
+    destruct reducer_sound as [ ? [ ? ? ] ].
+    rewrite H4 in *.
+    destruct (pctxD cs') eqn:?; auto.
+    destruct e'.
+    { simpl in *.
+      forward.
+      destruct H6; split; auto.
+      intros.
+      gather_facts.
+      eapply Pure_pctxD; eauto.
+      intros. rewrite H5. eauto. }
+    { simpl in *. rewrite H4 in *.
+      rewrite H3.
+      destruct H2; split; auto.
+      intros.
+      gather_facts.
+      eapply Pure_pctxD; eauto.
+      intros. rewrite H5.
+      auto. }
+  Qed.
+
+  Definition rw_post_simplify : lem_rewriter _ _ _ :=
+    Eval unfold rw_bind, rw_ret in
+      fun e r => rw_bind (lr e r)
+                         (fun e' => rw_ret match e' with
+                                           | Progress e' => Progress (reducer e')
+                                           | NoProgress => NoProgress
+                                           end).
+
+  Theorem rw_post_simplify_sound
+  : setoid_rewrite_spec RbaseD rw_post_simplify.
+  Proof using lr_sound reducer_sound.
+    unfold rw_post_simplify. do 2 red. intros.
+    forward. inv_all; subst.
+    eapply lr_sound in H1; eauto.
+    forward_reason; split; eauto.
+    intros. eapply H1 in H2; clear H1.
+    destruct (pctxD cs) eqn:?; auto.
+    destruct (lambda_exprD (getUVars ctx) (tvs' ++ getVars ctx) t e) eqn:?; auto.
+    destruct (pctxD cs') eqn:?; auto.
+    destruct p0; simpl in *.
+    { destruct (lambda_exprD (getUVars ctx) (tvs' ++ getVars ctx) t new_val) eqn:?; try contradiction.
+      eapply reducer_sound in Heqo2.
+      destruct Heqo2 as [ ? [ ? ? ] ].
+      rewrite H1. destruct H2; split; auto.
+      intros.
+      gather_facts.
+      eapply Pure_pctxD; eauto.
+      intros. rewrite <- H3. eauto. }
+    { destruct (lambda_exprD (getUVars ctx) (tvs' ++ getVars ctx) t e); auto. }
+  Qed.
+
+End setoid.
