theories/Lambda/Rewrite/Repeat.v
@@ -1,0 +1,196 @@
+Require Import Coq.Classes.Morphisms.
+Require Import Coq.Relations.Relations.
+Require Import ExtLib.Tactics.
+Require Import MirrorCore.SubstI.
+Require Import MirrorCore.Util.Forwardy.
+Require Import MirrorCore.Util.Compat.
+Require Import MirrorCore.Lambda.Expr.
+Require Import MirrorCore.Lambda.RewriteRelations.
+Require Import MirrorCore.Lambda.Rewrite.Core.
+
+Set Implicit Arguments.
+Set Strict Implicit.
+
+Set Suggest Proof Using.
+
+Section setoid.
+  Context {typ : Type}.
+  Context {func : Type}.
+  Context {RType_typD : RType typ}.
+  Context {Typ2_Fun : Typ2 RType_typD RFun}.
+  Context {RSym_func : RSym func}.
+
+  (** Reasoning principles **)
+  Context {RTypeOk_typD : RTypeOk}.
+  Context {Typ2Ok_Fun : Typ2Ok Typ2_Fun}.
+  Context {RSymOk_func : RSymOk RSym_func}.
+  Context {Typ0_Prop : Typ0 _ Prop}.
+
+  Local Existing Instance Subst_ctx_subst.
+  Local Existing Instance SubstOk_ctx_subst.
+  Local Existing Instance SubstUpdate_ctx_subst.
+  Local Existing Instance SubstUpdateOk_ctx_subst.
+  Local Existing Instance Expr_expr.
+  Local Existing Instance ExprOk_expr.
+
+  (* TODO(gmalecha): Wrap all of this up in a type class?
+   * Why should it be different than Expr?
+   *)
+  Variable Rbase : Type.
+  Variable Rbase_eq : Rbase -> Rbase -> bool.
+  Hypothesis Rbase_eq_ok : forall a b, Rbase_eq a b = true -> a = b.
+
+  Local Notation "'R'" := (R typ Rbase).
+
+  Variable RbaseD : Rbase -> forall t : typ, option (typD t -> typD t -> Prop).
+
+  (** Apply the same rewrite until it stops making progress
+   **)
+
+  Variable rw : lem_rewriter typ func Rbase.
+  Variable is_refl : refl_dec R.
+  Variable is_trans : trans_dec R.
+
+  Local Fixpoint repeat_rewrite' (n : nat)
+           (prog : expr typ func -> Progressing (expr typ func))
+           (e : expr typ func) (r : R)
+  : mrw typ func (Progressing (expr typ func)) :=
+    match n with
+    | 0 => if is_refl r
+           then rw_ret (prog e)
+           else rw_fail
+    | S n => rw_bind_catch
+               (rw e r)
+               (fun e' =>
+                  match e' with
+                  | NoProgress =>
+                    if is_refl r then rw_ret (prog e) else rw_fail
+                  | Progress e' as X =>
+                    if is_trans r then repeat_rewrite' n (@Progress _) e' r
+                    else rw_ret X
+                  end)
+               (if is_refl r
+                then rw_ret (prog e)
+                else rw_fail)
+    end.
+
+  Hypothesis rw_sound : setoid_rewrite_spec RbaseD rw.
+  Hypothesis is_reflOk : refl_dec_ok (RD RbaseD) is_refl.
+  Hypothesis is_transOk : trans_dec_ok (RD RbaseD) is_trans.
+
+  Local Lemma repeat_rewrite'_mono : forall n e r c A B C D E F X Y,
+      repeat_rewrite' (c:=c) n (@Progress _) e r A B C D E F = Some (X,Y) ->
+      X <> NoProgress.
+  Proof using.
+    induction n; simpl.
+    { intros. destruct (is_refl r). inversion H. congruence. inversion H. }
+    { intros.
+      eapply rw_bind_catch_case in H. destruct H; forward_reason.
+      { destruct x.
+        { destruct (is_trans r); eauto.
+          inversion H0. congruence. }
+        { destruct (is_refl r).
+          { inversion H0; congruence. }
+          { inversion H0. } } }
+      { destruct (is_refl r).
+        { inversion H; congruence. }
+        { inversion H. } } }
+  Qed.
+
+  Local Theorem repeat_rewrite'_sound
+  : forall n (prog : bool),
+      setoid_rewrite_spec
+        RbaseD
+        (repeat_rewrite' n
+                         (if prog then @Progress _ else (fun _ => NoProgress))).
+  Proof using is_reflOk is_transOk rw_sound.
+    induction n.
+    { intros. simpl. destruct prog.
+      { do 2 red. intros.
+        specialize (@is_reflOk r).
+        destruct (is_refl r).
+        { inversion H; clear H; subst.
+          split; auto.
+          intros.
+          eapply is_reflOk in H; trivial.
+          simpl.
+          forward.
+          split; [ reflexivity | ].
+          intros. eapply Pure_pctxD; eauto. }
+        { inversion H. } }
+      { do 2 red; intros.
+        specialize (@is_reflOk r).
+        destruct (is_refl r).
+        { inversion H; clear H; subst.
+          split; auto.
+          intros.
+          eapply is_reflOk in H; eauto.
+          simpl. forward.
+          split; [ reflexivity | ].
+          intros; eapply Pure_pctxD; eauto. }
+        { inversion H. } } }
+    { simpl. do 2 red; intros.
+      eapply rw_bind_catch_case in H; destruct H; forward_reason.
+      { eapply rw_sound in H.
+        forward_reason. destruct x.
+        { specialize (@is_transOk r).
+          destruct (is_trans r).
+          { generalize (repeat_rewrite'_mono _ _ _ _ _ _ _ _ _ H1).
+            eapply (IHn true) in H1.
+            forward_reason. split; auto.
+            intros.
+            specialize (H3 _ _ H5).
+            specialize (H2 _ _ H5).
+            simpl in *.
+            forward.
+            forward_reason.
+            destruct e'; simpl in *.
+            { Cases.rewrite_all_goal.
+              split; [ reflexivity | ].
+              intros. gather_facts.
+              eapply pctxD_SubstMorphism; [ | | eassumption | ]; eauto.
+              gather_facts.
+              eapply is_transOk in H5; eauto.
+              eapply Pure_pctxD; eauto. }
+            { congruence. } }
+          { inversion H1; clear H1; subst.
+            simpl in *. split; auto. } }
+        { specialize (@is_reflOk r).
+          destruct (is_refl r); [ | inversion H1 ].
+          inversion H1; clear H1; subst.
+          split; auto.
+          intros. specialize (H2 _ _ H1).
+          forward. destruct prog; simpl in *.
+          { rewrite H5. forward_reason.
+            split; auto. }
+          { rewrite H5; forward_reason; auto. } } }
+      { specialize (@is_reflOk r).
+        destruct (is_refl r); [ | inversion H ].
+        inversion H; clear H; subst.
+        split; auto.
+        intros.
+        forward.
+        cutrewrite (ProgressD e
+                              ((if prog then (@Progress _)
+                                else fun _ : expr typ func => NoProgress) e) = e);
+          [ | destruct prog; reflexivity ].
+        rewrite H3; forward_reason.
+        split; [ reflexivity | ].
+        eapply is_reflOk in H; eauto.
+        eapply Pure_pctxD; eauto. } }
+  Qed.
+
+  Definition repeat_rewrite (progress : bool)
+  : nat -> lem_rewriter typ func Rbase :=
+    let prog := if progress then @Progress _ else (fun _ => NoProgress) in
+    fun n =>
+      repeat_rewrite' n prog.
+
+  Theorem repeat_rewrite_sound
+  : forall b n, setoid_rewrite_spec RbaseD (repeat_rewrite b n).
+  Proof using is_reflOk is_transOk rw_sound.
+    unfold repeat_rewrite. simpl. intros.
+    eapply repeat_rewrite'_sound.
+  Qed.
+
+End setoid.
