theories/Lambda/Rewrite/Respectful.v
@@ -1,0 +1,337 @@
+Require Import Coq.Classes.Morphisms.
+Require Import Coq.Relations.Relations.
+Require Import ExtLib.Core.RelDec.
+Require Import ExtLib.Data.HList.
+Require Import ExtLib.Tactics.
+Require Import MirrorCore.SubstI.
+Require Import MirrorCore.Lemma.
+Require Import MirrorCore.VarsToUVars.
+Require Import MirrorCore.Instantiate.
+Require Import MirrorCore.Util.Forwardy.
+Require Import MirrorCore.Util.Compat.
+Require Import MirrorCore.Util.Iteration.
+Require Import MirrorCore.RTac.Core.
+Require Import MirrorCore.RTac.CoreK.
+Require Import MirrorCore.Lambda.Expr.
+Require Import MirrorCore.Lambda.ExprTac.
+Require Import MirrorCore.Lambda.ExprUnify.
+Require Import MirrorCore.Lambda.AppN.
+Require Import MirrorCore.Lambda.ExprSubstitute.
+Require Import MirrorCore.Lambda.RewriteRelations.
+Require Import MirrorCore.Lambda.Rewrite.Core.
+
+Set Implicit Arguments.
+Set Strict Implicit.
+
+Set Suggest Proof Using.
+
+Section setoid.
+  Context {typ : Type}.
+  Context {func : Type}.
+  Context {RType_typD : RType typ}.
+  Context {Typ2_Fun : Typ2 RType_typD RFun}.
+  Context {RSym_func : RSym func}.
+
+  (** Reasoning principles **)
+  Context {RTypeOk_typD : RTypeOk}.
+  Context {Typ2Ok_Fun : Typ2Ok Typ2_Fun}.
+  Context {RSymOk_func : RSymOk RSym_func}.
+  Context {Typ0_Prop : Typ0 _ Prop}.
+
+  Context {RelDec_eq_typ : RelDec (@eq typ)}.
+  Context {RelDec_Correct_eq_typ : RelDec_Correct RelDec_eq_typ}.
+
+  Local Existing Instance Subst_ctx_subst.
+  Local Existing Instance SubstOk_ctx_subst.
+  Local Existing Instance SubstUpdate_ctx_subst.
+  Local Existing Instance SubstUpdateOk_ctx_subst.
+  Local Existing Instance Expr_expr.
+  Local Existing Instance ExprOk_expr.
+
+  (* TODO(gmalecha): Wrap all of this up in a type class?
+   * Why should it be different than Expr?
+   *)
+  Variable Rbase : Type.
+  Variable Rbase_eq : Rbase -> Rbase -> bool.
+  Hypothesis Rbase_eq_ok : forall a b, Rbase_eq a b = true -> a = b.
+
+  Local Notation "'R'" := (R typ Rbase).
+
+  Variable RbaseD : Rbase -> forall t : typ, option (typD t -> typD t -> Prop).
+
+  Hypothesis RbaseD_single_type
+  : forall r t1 t2 rD1 rD2,
+      RbaseD r t1 = Some rD1 ->
+      RbaseD r t2 = Some rD2 ->
+      t1 = t2.
+
+  (** This starts plugins for the rewriter **)
+  (******************************************)
+
+  Definition func_sdec (a b : func) : bool :=
+    match sym_eqb a b with
+    | Some x => x
+    | _ => false
+    end.
+
+  Definition expr_sdec : expr typ func -> expr typ func -> bool :=
+    @expr_eq_sdec typ func _ func_sdec.
+
+  Lemma expr_sdec_sound
+  : forall a b : expr typ func, expr_sdec a b = true -> a = b.
+  Proof using RSymOk_func RelDec_Correct_eq_typ.
+    eapply expr_eq_sdec_ok; eauto.
+    unfold func_sdec.
+    intros. generalize (sym_eqbOk a b); eauto with typeclass_instances.
+    destruct (sym_eqb a b); intros; subst; auto.
+    inversion H.
+  Qed.
+
+  (* This is just a "special" version of the rewriting lemma *)
+  Record Proper_concl : Type :=
+  { relation : R
+  ; term     : expr typ func
+  }.
+
+  Definition Proper_conclD (tus tvs : tenv typ) (p : Proper_concl)
+  : option (exprT tus tvs Prop) :=
+    match typeof_expr tus tvs p.(term) with
+    | Some t =>
+      match RD RbaseD p.(relation) t
+            , lambda_exprD tus tvs t p.(term)
+      with
+      | Some rD , Some eD =>
+        Some (fun us vs => rD (eD us vs) (eD us vs))
+      | _ , _ => None
+      end
+    | None => None
+    end.
+
+  Definition Proper_lemma := Lemma.lemma typ (expr typ func) Proper_concl.
+
+  (* This splits a relation into a relation arity and a relation *)
+  Local Fixpoint split_R (r : R) : list R * R :=
+    match r with
+    | Rrespects l r =>
+      let (ls, r) := split_R r in
+      (l :: ls, r)
+    | _ => (nil, r)
+    end.
+
+  Local Lemma split_R_sound : forall r_end r rs,
+      split_R r = (rs, r_end) ->
+      fold_right Rrespects r_end rs = r.
+  Proof using.
+    induction r; simpl; intros; inv_all; subst; simpl; try reflexivity.
+    destruct (split_R r2). inv_all. subst.
+    specialize (IHr2 _ eq_refl).
+    simpl. rewrite IHr2. reflexivity.
+  Qed.
+
+  Require Import MirrorCore.RTac.CoreK.
+
+  Definition apply_respectful (lem : Proper_lemma)
+             (tacK : rtacK typ (expr typ func))
+  : respectful_dec _ _ _ :=
+    let (rs,r_final) := split_R lem.(Lemma.concl).(relation) in
+    match lem.(Lemma.vars) with
+    | nil => match lem.(Lemma.premises) with
+             | nil => fun e r =>
+                        match expr_sdec e lem.(Lemma.concl).(term)
+                            , Req_dec Rbase_eq r r_final
+                        with
+                        | true , true => rw_ret rs
+                        | _ , _ => rw_fail
+                        end
+             | _ :: _ => fun e r =>
+                           (** TODO(gmalecha): Handle this *)
+                           rw_fail
+             end
+    | _ :: _ => fun _ _ => (** TODO(gmalecha): Handle this *)
+                  rw_fail
+    end.
+
+  Theorem apply_respectful_sound : forall lem tacK,
+      Lemma.lemmaD Proper_conclD nil nil lem ->
+      forall Htac : rtacK_sound tacK,
+        respectful_spec RbaseD (apply_respectful lem tacK).
+  Proof using RSymOk_func RTypeOk_typD Rbase_eq_ok RelDec_Correct_eq_typ
+        Typ2Ok_Fun.
+    red; intros.
+    unfold apply_respectful in H0.
+    consider (split_R (relation (Lemma.concl lem))); intros.
+    destruct (Lemma.vars lem) eqn:?.
+    { destruct (Lemma.premises lem) eqn:?; try solve [ inversion H2 ].
+      generalize (expr_sdec_sound e lem.(Lemma.concl).(term)).
+      generalize (Req_dec_ok Rbase_eq Rbase_eq_ok r r0).
+      destruct (expr_sdec e (term (Lemma.concl lem))); try solve [ inversion H2 ].
+      destruct (Req_dec Rbase_eq r r0); try solve [ inversion H2 ].
+      unfold rw_ret in H2. inv_all.
+      intros. specialize (H2 eq_refl). specialize (H5 eq_refl).
+      subst.
+      split; auto. intros.
+      forward.
+      red in H.
+      simpl in H.
+      unfold Lemma.lemmaD' in H.
+      forwardy. inv_all. subst.
+      generalize dependent lem.(Lemma.vars); intros; subst.
+      generalize dependent lem.(Lemma.premises); intros; subst.
+      simpl in *.
+      unfold Proper_conclD in H6.
+      forwardy.
+      inv_all. subst.
+      simpl in *.
+      erewrite split_R_sound by eassumption.
+      destruct (ExprFacts.lambda_exprD_weaken _ _ _ (getUVars ctx) (tvs'++getVars ctx) H8) as [ ? [ ? ? ] ].
+      simpl in H.
+      generalize (@lambda_exprD_deterministic _ _ _ _ _ _ _ _ _ _ _ _ _ _ _ H H4).
+      unfold Rty. intros.
+      revert H5.
+      subst y. intros.
+      rewrite H7.
+      split; [ reflexivity | ].
+      intros.
+      eapply Pure_pctxD; eauto.
+      intros.
+      specialize (@H9 HList.Hnil HList.Hnil us0 (HList.hlist_app vs' vs0)); simpl in H9.
+      rewrite H9 in H5.
+      rewrite H4 in H.
+      inv_all. subst. eapply H5. }
+    { inversion H2. }
+  Qed.
+
+  Definition apply_prespectful {T : Type}
+             (get : expr typ func -> R -> option T)
+             (lem : T -> Proper_lemma) (tacK : rtacK _ _)
+    : respectful_dec _ _ _ :=
+    fun e r =>
+      match get e r with
+      | Some t => apply_respectful (lem t) tacK e r
+      | _ => rw_fail
+      end.
+
+  Theorem apply_prespectful_sound : forall {T} get (lem : T -> _) (tacK : _),
+      (forall e r x,
+          get e r = Some x ->
+          forall tus tvs t eD,
+            lambda_exprD tus tvs t e = Some eD ->
+            Lemma.lemmaD Proper_conclD nil nil (lem x)) ->
+      rtacK_sound tacK ->
+      respectful_spec RbaseD (apply_prespectful get lem tacK).
+  Proof using RSymOk_func RTypeOk_typD Rbase_eq_ok RelDec_Correct_eq_typ
+        Typ2Ok_Fun.
+    intros. unfold apply_prespectful.
+    red. intros.
+    destruct (get e r) eqn:?; try solve [ inversion H1 ].
+    (** above *)
+    unfold apply_respectful in H1.
+    destruct (split_R t.(lem).(concl).(relation)) eqn:?.
+    eapply split_R_sound in Heqp.
+    destruct (t.(lem).(vars)) eqn:Hvars; [ | inversion H1 ].
+    destruct (t.(lem).(premises)) eqn:Hprems; [ | inversion H1 ].
+    generalize (expr_sdec_sound e t.(lem).(concl).(term)).
+    destruct (expr_sdec e t.(lem).(concl).(term)); [ | inversion H1 ].
+    generalize (Req_dec_ok _ Rbase_eq_ok r r0).
+    destruct (Req_dec Rbase_eq r r0); [ | inversion H1 ].
+    intro X; specialize (X eq_refl); subst.
+    intro X; specialize (X eq_refl); subst.
+    inversion H1; clear H1; subst.
+    split; auto.
+    intros.
+    forward.
+    eapply H in Heqo; [ | eapply H4 ].
+    rename Heqo into Hlem.
+    red in Hlem.
+    simpl in Hlem.
+    red in Hlem. rewrite Hprems in *. rewrite Hvars in *.
+    simpl in Hlem. red in Hlem.
+    revert Hlem.
+    forward. inv_all. subst.
+    destruct (ExprFacts.lambda_exprD_weaken _ _ _ (getUVars ctx) (tvs'++getVars ctx) H8) as [ ? [ ? ? ] ].
+    simpl in H.
+    generalize (@lambda_exprD_deterministic _ _ _ _ _ _ _ _ _ _ _ _ _ _ _ H6 H4).
+    intro. red in H10. revert Hlem. subst.
+    simpl in *.
+    rewrite Heqp in *.
+    rewrite H7 in *.
+    rewrite H4 in *.
+    inv_all. subst.
+    intros.
+    intros; split; [ reflexivity | ].
+    intros. eapply Pure_pctxD; eauto.
+    intros. red.
+    rewrite (H9 Hnil Hnil us0 (hlist_app vs' vs0)) in Hlem.
+    eapply Hlem.
+  Qed.
+
+  Definition or_respectful
+             (a b : expr typ func -> R -> mrw typ func (list R))
+    : respectful_dec _ _ _ :=
+    fun e r => rw_orelse (a e r) (b e r).
+
+  Theorem or_respectful_sound : forall a b,
+      respectful_spec RbaseD a ->
+      respectful_spec RbaseD b ->
+      respectful_spec RbaseD (or_respectful a b).
+  Proof using.
+    unfold or_respectful. intros.
+    red. intros.
+    eapply rw_orelse_case in H1; destruct H1; [ eapply H | eapply H0 ];
+      eassumption.
+  Qed.
+
+  Definition fail_respectful : respectful_dec typ func Rbase :=
+    fun _ _ => rw_fail.
+
+  Theorem fail_respectful_sound : respectful_spec RbaseD fail_respectful.
+  Proof using.
+    red. intros. inversion H.
+  Qed.
+
+  Require Import MirrorCore.RTac.IdtacK.
+
+  Fixpoint do_respectful (propers : list (expr typ func * R))
+    : respectful_dec _ _ _ :=
+    match propers with
+    | nil => fail_respectful
+    | (f,rel) :: propers =>
+      or_respectful
+        (apply_respectful {| vars := nil
+                             ; premises := nil
+                             ; concl := {| relation := rel
+                                           ; term := f |}
+                          |} IDTACK)
+        (fun x => do_respectful propers x)
+    end.
+
+  Theorem do_respectful_sound
+    : forall propers,
+      Forall (fun er =>
+                let '(e,r) := er in
+                match typeof_expr nil nil e with
+                | None => False
+                | Some t =>
+                  match RD RbaseD r t
+                        , lambda_exprD nil nil t e
+                  with
+                  | Some rD , Some eD =>
+                    Proper rD (eD Hnil Hnil)
+                  | _ , _ => False
+                  end
+                end) propers ->
+      respectful_spec RbaseD (do_respectful propers).
+  Proof using RTypeOk_typD Typ2Ok_Fun RSymOk_func RelDec_Correct_eq_typ Rbase_eq_ok.
+    induction 1.
+    { eapply fail_respectful_sound. }
+    { simpl. destruct x. eapply or_respectful_sound.
+      { apply apply_respectful_sound.
+        { clear - H.
+          red. simpl. unfold lemmaD'. simpl.
+          unfold Proper_conclD. simpl.
+          forward. }
+        { apply IDTACK_sound. } }
+      { eauto. } }
+  Qed.
+
+End setoid.
