theories/Lambda/Rewrite/Tactic.v
@@ -1,0 +1,156 @@
+Require Import Coq.omega.Omega.
+Require Import Coq.Classes.Morphisms.
+Require Import Coq.PArith.BinPos.
+Require Import Coq.Relations.Relations.
+Require Import Coq.FSets.FMapPositive.
+Require Import ExtLib.Core.RelDec.
+Require Import ExtLib.Data.Positive.
+Require Import ExtLib.Data.List.
+Require Import ExtLib.Data.HList.
+Require Import ExtLib.Data.Option.
+Require Import ExtLib.Data.Pair.
+Require Import ExtLib.Recur.Relation.
+Require Import ExtLib.Recur.GenRec.
+Require Import ExtLib.Recur.Facts.
+Require Import ExtLib.Tactics.
+Require Import MirrorCore.SubstI.
+Require Import MirrorCore.Lemma.
+Require Import MirrorCore.VarsToUVars.
+Require Import MirrorCore.Instantiate.
+Require Import MirrorCore.Util.Forwardy.
+Require Import MirrorCore.Util.Compat.
+Require Import MirrorCore.Util.Iteration.
+Require Import MirrorCore.RTac.Core.
+Require Import MirrorCore.RTac.CoreK.
+Require Import MirrorCore.Lambda.Expr.
+Require Import MirrorCore.Lambda.ExprTac.
+Require Import MirrorCore.Lambda.ExprUnify.
+Require Import MirrorCore.Lambda.AppN.
+Require Import MirrorCore.Lambda.ExprSubstitute.
+Require Import MirrorCore.Lambda.RewriteRelations.
+Require Import MirrorCore.Lambda.Rewrite.Core.
+Require Import MirrorCore.Lambda.Rewrite.BottomUp.
+
+Set Implicit Arguments.
+Set Strict Implicit.
+
+Set Suggest Proof Using.
+
+Section setoid.
+  Context {typ : Type}.
+  Context {func : Type}.
+  Context {RType_typD : RType typ}.
+  Context {Typ2_Fun : Typ2 RType_typD RFun}.
+  Context {RSym_func : RSym func}.
+
+  (** Reasoning principles **)
+  Context {RTypeOk_typD : RTypeOk}.
+  Context {Typ2Ok_Fun : Typ2Ok Typ2_Fun}.
+  Context {RSymOk_func : RSymOk RSym_func}.
+  Context {Typ0_Prop : Typ0 _ Prop}.
+
+  (** TODO(gmalecha): This is not necessary *)
+  Context {RelDec_eq_typ : RelDec (@eq typ)}.
+  Context {RelDec_Correct_eq_typ : RelDec_Correct RelDec_eq_typ}.
+
+  (* TODO(gmalecha): Wrap all of this up in a type class?
+   * Why should it be different than Expr?
+   *)
+  Variable Rbase : Type.
+  Variable Rbase_eq : Rbase -> Rbase -> bool.
+  Hypothesis Rbase_eq_ok : forall a b, Rbase_eq a b = true -> a = b.
+
+  Local Notation "'R'" := (R typ Rbase).
+
+  Variable RbaseD : Rbase -> forall t : typ, option (typD t -> typD t -> Prop).
+
+  Hypothesis RbaseD_single_type
+  : forall r t1 t2 rD1 rD2,
+      RbaseD r t1 = Some rD1 ->
+      RbaseD r t2 = Some rD2 ->
+      t1 = t2.
+
+  Local Existing Instance Subst_ctx_subst.
+  Local Existing Instance SubstOk_ctx_subst.
+  Local Existing Instance SubstUpdate_ctx_subst.
+  Local Existing Instance SubstUpdateOk_ctx_subst.
+  Local Existing Instance Expr_expr.
+  Local Existing Instance ExprOk_expr.
+
+
+  Definition auto_setoid_rewrite_bu
+             (r : R)
+             (reflexive : refl_dec R)
+             (transitive : trans_dec R)
+             (rewriter : lem_rewriter typ func Rbase)
+             (respectful : respectful_dec typ func Rbase)
+  : rtac typ (expr typ func) :=
+    let rw := bottom_up reflexive transitive rewriter respectful in
+    fun tus tvs nus nvs ctx cs g =>
+      match @rw g r nil tus tvs nus nvs ctx cs with
+      | None => Fail
+      | Some (Progress g', cs') => More_ cs' (GGoal g')
+      | Some (NoProgress, cs') => Fail
+      end.
+
+  Variable R_impl : R.
+
+  Hypothesis R_impl_is_impl
+    : RD RbaseD R_impl (typ0 (F:=Prop)) =
+      Some match eq_sym (typ0_cast (F:=Prop)) in _ = t return t -> t -> Prop with
+           | eq_refl => Basics.impl
+           end.
+
+  Theorem auto_setoid_rewrite_bu_sound
+  : forall is_refl is_trans rw proper
+           (His_reflOk : refl_dec_ok (RD RbaseD) is_refl)
+           (His_transOk : trans_dec_ok (RD RbaseD) is_trans),
+      setoid_rewrite_spec RbaseD rw ->
+      respectful_spec RbaseD  proper ->
+      rtac_sound (auto_setoid_rewrite_bu (Rflip R_impl)
+                                         is_refl is_trans rw proper).
+  Proof using RSymOk_func RTypeOk_typD R_impl_is_impl
+        RbaseD_single_type Typ2Ok_Fun.
+    intros. unfold auto_setoid_rewrite_bu. red.
+    intros.
+    generalize (@bottom_up_sound _ _ _ _ _ _ _ _ _ _ _
+                                 RbaseD_single_type is_refl is_trans rw proper
+                                 His_reflOk His_transOk H H0 g (Rflip R_impl) ctx s nil).
+    simpl.
+    destruct (bottom_up is_refl is_trans rw proper g (Rflip R_impl) nil
+      (getUVars ctx) (getVars ctx) (length (getUVars ctx))
+      (length (getVars ctx)) s).
+    { destruct p. destruct p; subst; eauto using rtac_spec_Fail.
+      red. intros Hbus ? ?.
+      specialize (Hbus _ _ eq_refl H2).
+      forward_reason.
+      split; try assumption.
+      split; [ constructor | ].
+      specialize (H4 (typ0 (F:=Prop))).
+      rewrite R_impl_is_impl in H4.
+      specialize (H4 _ eq_refl).
+      revert H4.
+      destruct (pctxD s) eqn:HpctxDs; try (clear; tauto).
+      simpl. unfold propD. unfold exprD_typ0.
+      simpl.
+      destruct (lambda_exprD (getUVars ctx) (getVars ctx) (typ0 (F:=Prop)) g);
+        try solve [ tauto ].
+      destruct (pctxD c) eqn:HpctxDc; try solve [ tauto ].
+      destruct (lambda_exprD (getUVars ctx) (getVars ctx) (typ0 (F:=Prop)) new_val);
+        try solve [ tauto ].
+      destruct 1; split; try assumption.
+      intros.
+      gather_facts.
+      eapply Pure_pctxD; eauto.
+      intros.
+      specialize (H5 Hnil). simpl in *.
+      revert H6 H5. autorewrite_with_eq_rw.
+      clear. generalize (typ0_cast (F:=Prop)).
+      generalize dependent (typD (typ0 (F:=Prop))).
+      do 4 intro. subst. simpl.
+      unfold flip, Basics.impl. tauto. }
+    { subst. intro. clear.
+      eapply rtac_spec_Fail. }
+  Qed.
+
+End setoid.
