theories/Lambda/RewriteStrat.v
@@ -1,0 +1,9 @@
+Require Export MirrorCore.Lambda.RewriteRelations.
+Require Export MirrorCore.Lambda.Rewrite.Core.
+Require Export MirrorCore.Lambda.Rewrite.BottomUp.
+Require Export MirrorCore.Lambda.Rewrite.Repeat.
+Require Export MirrorCore.Lambda.Rewrite.Respectful.
+Require Export MirrorCore.Lambda.Rewrite.Reduce.
+Require Export MirrorCore.Lambda.Rewrite.Rewrite.
+Require Export MirrorCore.Lambda.Rewrite.HintDbs.
+Require Export MirrorCore.Lambda.Rewrite.Tactic.
